meta_subst.v
@@ -2,10 +2,7 @@ Require Import util.
 Require Import worlds. 
 Require Import meta_term.
 
-Definition mbind D D1 D2 := (slink D1 D2)*(meta_term D).
-Definition msubst D R := star (mbind R) empty D.
-Definition msubst_cons D R := @s_cons _ (mbind R) empty D.
-Implicit Arguments msubst_cons.
+Definition msubst δ δ' := name δ -> meta_term δ'.
 Class substitutable (A:world -> Set) := 
    app_subst : forall {α β}, msubst α β -> A α -> A β.
 Notation "⟦ θ ⟧" := (app_subst θ). 
@@ -13,6 +10,3 @@ Typeclasses Transparent substitutable.
 Typeclasses Transparent app_subst.
 
 Hint Transparent app_subst.
-
-(* Uh oh, termination of substitution depends on types.
-    It's actually not possible (rather, ugly) to implement as-is. *)
