meta_subst_type.v
@@ -7,16 +7,12 @@ Require Import meta_subst_meta_term.
 Require Import meta_subst_typing.
 Require Import meta_term.
 
- 
-Fixpoint import_msubst {δ δ' δ''} (X:δ'↪δ'')  (θ:msubst δ δ')  : msubst δ δ'' :=
-match θ in star _ _ δ return star (mbind δ'') empty δ with
- | · => ·
- | (θ',, (Y,t)) => import_msubst X θ',, (Y, import_meta_term X t)
-end.
+
+Definition import_msubst {δ δ' δ''} (X:δ'↪δ'')  (θ:msubst δ δ')  : msubst δ δ'' :=
+ import_meta_term X ○ θ.
 
 Section app_msubst_t2_sect.
 
-Notation "θ ;; X' // X" := ((import_msubst X' θ) ; (m_var X') // X) (at level 90).
 Reserved Notation "[ θ ] T" (at level 90).
 
 Fixpoint app_msubst_t2 {ψ} {δ δ'} (θ:msubst δ δ') (T:tp' ψ δ) : tp' ψ δ' :=
@@ -27,10 +23,10 @@ match T  with
    arr ([θ] T1) ([θ] T2)
  | pi _ X U T0 =>
    let (_,X') := next δ' in
-   pi X' (⟦θ⟧ U) ([θ;;X'//X] T0)
+   pi X' (⟦θ⟧ U) ([import_msubst X' θ,, (X,m_var X')] T0)
  | sigma _ X U T0 =>
    let (_,X') := next δ' in
-   sigma X' (⟦θ⟧ U) ([θ;;X'//X] T0)
+   sigma X' (⟦θ⟧ U) ([import_msubst X' θ,, (X,m_var X')] T0)
  | unit =>
    unit _ _
  | prod T1 T2 =>
@@ -48,6 +44,8 @@ where "[ θ ] T" := (app_msubst_t2 θ T).
 End app_msubst_t2_sect.
 Implicit Arguments app_msubst_t2.
 
+
+ Instance tp_substitutable : substitutable tp := (@app_msubst_t2 empty).
 
 Axiom msubst_single_t : forall {D D'} (X:wlink D D'), meta_term D -> tp D' -> tp D.
 (* TODO: Write this as a simultaneous substitution: (id,C/X) ? *)
