util.v
@@ -1,12 +1,48 @@
-Section star.
+(*Section star.
  Hypotheses (A:Set) (Rel:A -> A -> Set).
  Inductive star (a:A) : A -> Set :=
   | s_nil : star a a
   | s_cons : forall b c, star a b -> Rel b c -> star a c.
- End star.
+End star.
  Implicit Arguments star.
  Implicit Arguments s_nil.
  Implicit Arguments s_cons.
  Print Implicit s_cons.
- Implicit Arguments s_nil [A Rel a].
- Notation "A ,, B" := (s_cons _ A B) (at level 90).
+ Implicit Arguments s_nil [A Rel a]. *)
+ Require Import worlds.
+ Require Import Coq.Logic.FunctionalExtensionality.
+ Definition cdot {A} : name empty -> A := fun n => match (empty_is_empty n) with end.
+ Notation "·" := cdot.
+
+ Definition maybe {A C} (f:A -> C) (c:C) (x:A + unit) : C := match x with | inl a => f a | inr _ => c end.  
+
+Definition compose
+  {A:Set}
+  {B:Set}
+  {C:Set}
+  (f:A -> B)
+  (g:B -> C)
+  (a:A) : C
+ := g (f a). 
+ Notation "f ○ g" := (compose g f) (at level 10).
+
+ Notation "Γ ,, ( y , t )" := ((maybe Γ t) ○ (export y)) (at level 90).
+
+Lemma compose_assoc {A B C D:Set} (f:A -> B) (g:B -> C) (h:C -> D) : (h ○ g) ○ f = h ○ (g ○ f).
+eapply functional_extensionality. 
+intro. unfold compose.
+reflexivity.
+Qed.
+
+Lemma f_maybe {A B C:Set} (f:B -> C) (Γ:A -> B) (t:B) :
+ f ○ (maybe Γ t) = maybe (f ○ Γ) (f t).  
+eapply functional_extensionality; intro. unfold compose.
+destruct x; simpl; reflexivity.
+Qed.
+
+Lemma compose_comma {α β} {x:α↪β} {B C:Set} (f:B -> C)
+ (Γ:name α -> B) (b:B) :
+ f ○ (Γ,, (x,b)) = (f ○ Γ,, (x,f b)). 
+erewrite <- compose_assoc.
+erewrite f_maybe. reflexivity.
+Qed.
