meta_subst_meta_term.v
@@ -6,15 +6,7 @@ Require Import meta_subst_typing.
 
 Axiom app_msubst : forall W W', msubst W W' -> meta_term W -> meta_term W'.
 
-Fixpoint app_msubst_mvar {δ δ'} (θ:msubst δ δ') : name δ -> meta_term δ' := 
-match θ in star _ _ δ return name δ -> meta_term δ' with
-| · => fun n => match (empty_is_empty n) with end
-| (θ',,(Y,t)) => fun n =>
-  match (export Y n) with
-   | inleft n0 => app_msubst_mvar θ' n0
-   | inright _ => t
-  end
-end.
+Definition app_msubst_mvar {δ δ'} (θ:msubst δ δ') : name δ -> meta_term δ' := fun n => θ n.
 
 Implicit Arguments app_msubst.
 Instance meta_term_substitutable : substitutable meta_term :=
