meta_subst_typing.v
@@ -4,16 +4,14 @@ Require Import meta_subst.
 Require Import meta_term.
 Require Import meta_subst_meta_type.
  Reserved Notation "D ⊩ T ∷ D2" (at level 90).
- Notation "T ;  t // y " := (msubst_cons T (y,t)) (at level 90).
- Notation "·" := (s_nil).
 
  Inductive msubst_typ' {α}(Δ:mtype_assign α) : forall {β}(Δ':mtype_assign β), msubst β α ->Prop :=
   | m_subst_typ_nil :
            Δ ⊩ · ∷ ·
-  | m_subst_typ_cons : forall β Δ' γ (y:β ↪ γ) U t θ,
+  | m_subst_typ_cons : forall β γ (Δ':mtype_assign β) (y:β ↪ γ) (U:mtype β) (t:meta_term α) (θ:msubst β α),
            Δ ⊩ θ ∷ Δ' 
         -> Δ ⊨ t ∷ (⟦θ⟧ U)
-        -> Δ ⊩ (θ; t//y) ∷ (Δ',,(y,U))
+        -> Δ ⊩ (θ,, (y,t)) ∷ (import_mtype y ○ (Δ',,(y,U)))
   where "D ⊩ T ∷ D2" := (@msubst_typ' _ D _ D2 T).
  
 Definition msubst_typ {α} (Δ:mtype_assign α) {β} (Δ':mtype_assign β) θ := msubst_typ' Δ' Δ θ.
