meta_term.v
@@ -11,27 +11,10 @@ Require Import util.
  Axiom import_mtype : forall {δ δ'}, δ↪δ' -> mtype δ -> mtype δ'.
 
  Open Scope type_scope.
- Definition var_mtp D1 D2 := (slink D1 D2)*(mtype D1).
- Definition mtype_assign := star var_mtp empty.
+ Definition mtype_assign δ := name δ -> mtype δ.
 
- 
- (* This is basically the "In" predicate, except that we import things to the end *)
- Inductive m_assigned D : mtype_assign D -> name D -> mtype D -> Prop :=
-  | m_asn_top : forall D' (A:mtype_assign D') T x,
-                    m_assigned D (A,,(x,T)) x (import_mtype x T)
-  | m_asn_else : forall D' T A x (y:slink D' D) U,
-                 m_assigned D' A x T
-                 -> m_assigned D (A,,(y,U)) (import y x) (import_mtype y T). 
- Implicit Arguments m_assigned.
- Implicit Arguments m_asn_top.
- Implicit Arguments m_asn_else.
-
- Axiom m_oft : forall {D':world} {D:mtype_assign D'}, meta_term D' -> mtype D' -> Prop.
- (*  m_var_tp : forall y T, m_assigned D y T -> m_oft y T *)
-
-
+ Axiom m_oft : forall {δ:world} {Δ:mtype_assign δ}, meta_term δ -> mtype δ -> Prop.
  Implicit Arguments m_oft.
 
  Notation "D ⊨ t ∷ U" := (m_oft D t U) (at level 90).
- (* wf_mtype A T if T is a well-formed meta-type in the context A *)
 
