worlds.v
@@ -14,5 +14,6 @@ Parameter world : Set.
  Definition next a : {b:world & a↪b} := existT _ (projT1 (next' a)) (projT2 (next' a)).
  Axiom import_inj : forall {α β} {y:α↪β} {x x0}, import y x = import y x0 -> x = x0. 
  Axiom import_img : forall {α β} (y:α↪β) x, import y x <> y.
- Parameter export : forall {α β} (y:α↪β) (n:name β), name α + {n = y}.
- Axiom export_exclusive : forall {α β} {y:α↪β} {n:name α}, inleft _ n = export y y -> False.
+ Parameter export : forall {α β} (y:α↪β) (n:name β), name α + unit.
+ Axiom export_exclusive : forall {α β} {y:α↪β} {n:name α}, inl _ n = export y y -> False.
+ Axiom empty_fst : forall {α}, α↪empty -> False.
